More progress

Test/dafny0/ExternValiditySingletons.dfy
@@ -6,7 +6,7 @@ module ExternalInvariants {
     predicate Valid() 
       reads this, Repr 
       ensures Valid() ==> this in Repr
-      ensures Valid() ==> forall v :: v in Repr ==> v.Repr <= Repr
+      ensures Valid() ==> forall v :: v in Repr ==> v in AllValidatables() && v.Repr <= Repr
       ensures Valid() ==> forall v :: v in Repr && v != this ==> this !in v.Repr
     predicate P() {
       true
@@ -15,11 +15,12 @@ module ExternalInvariants {
     twostate lemma AllStillValid() 
       requires old(AllValid())
       requires Valid()
+      requires unchanged(AllValidatables())
       requires forall o :: o !in Repr ==> unchanged(o)
       requires forall o :: o in Repr ==> o.Valid()
       ensures AllValid()
     {
-      forall v: Validatable | v in AllExternallyValid() && old(allocated(v)) && v.P() ensures v.Valid() {
+      forall v | v in AllValidatables() && old(allocated(v)) ensures v.Valid() {
         IndependentValidityInductive(v, Repr);
       }
     }
@@ -31,16 +32,13 @@ module ExternalInvariants {
       ensures Valid()
   }
 
-  function {:extern} AllExternallyValid(): set<Validatable>
+  function AllValidatables(): set<Validatable>
 
   method {:extern} RegisterExternallyValid(v: Validatable)
-    requires v !in AllExternallyValid()
-    ensures AllExternallyValid() == old(AllExternallyValid()) + {v}
+    ensures AllValidatables() == old(AllValidatables()) + {v}
 
-  method {:extern} UnregisterExternallyValid(v: Validatable)
-    requires v in AllExternallyValid()
-    ensures AllExternallyValid() == old(AllExternallyValid()) - {v}
-
+  twostate lemma {:axiom} AllValidatablesUnchanged() 
+    ensures unchanged(AllValidatables())
 
   // This is the "external invariant". It must hold as a precondition and postcondition for
   // every method that crosses the Dafny/external boundary, either incoming or outgoing.
@@ -48,30 +46,21 @@ module ExternalInvariants {
   // I have to pass in the set of objects implementing Validatable since I can't pass in
   // "the Dafny heap".
   predicate AllValid() 
-    reads AllExternallyValid()
-    reads set v, o | v in AllExternallyValid() && o in v.Repr :: o
+    reads AllValidatables()
+    reads set v, o | v in AllValidatables() && o in v.Repr :: o
   {
-    forall v :: v in AllExternallyValid() ==> v.Valid()
+    forall v :: v in AllValidatables() ==> v.Valid()
   }
-
-  twostate lemma Validity(v: Validatable) 
-    requires old(AllValid())
-    requires v in old(AllExternallyValid())
-    ensures old(v.Valid())
-  {}
 
   twostate lemma IndependentValidityInductive(v: Validatable, changed: set<Validatable>)
       requires old(AllValid())
-      requires v in AllExternallyValid()
-      requires unchanged(AllExternallyValid())
+      requires v in AllValidatables()
       requires forall o :: o !in changed ==> unchanged(o)
       requires forall o :: o in changed ==> o.Valid()
       requires allocated(v)
       decreases v.Repr
       ensures v.Valid()
   {
-    Validity(v);
-    assert old(v.Valid());
     forall v': Validatable | v' in v.Repr && v' != v && old(allocated(v')) ensures v'.Valid() {
       IndependentValidityInductive(v', changed);
     }
@@ -87,22 +76,27 @@ module ExternalInvariants {
 
     constructor(x: int) 
       ensures Valid() 
-      ensures forall o: Validatable :: allocated(o) && fresh(o) && o.P() ==> o.Valid()
       ensures fresh(Repr)
+      ensures AllValidatables() - old(AllValidatables()) == {this}
     {
       this.x := x;
       this.y := 2*x;
       this.Repr := {this};
+      new;
+      
+      AllValidatablesUnchanged();
+      RegisterExternallyValid(this);
     }
     
     predicate Valid() 
       reads this, Repr 
       ensures Valid() ==> this in Repr
-      ensures Valid() ==> forall v :: v in Repr ==> v.Repr <= Repr
+      ensures Valid() ==> forall v :: v in Repr ==> v in AllValidatables() && v.Repr <= Repr
       ensures Valid() ==> forall v :: v in Repr && v != this ==> this !in v.Repr
     {
       && y == 2*x
       && Repr == {this}
+      && this in AllValidatables()
     }
     twostate lemma IndependentValidity()
       requires old(Valid())
@@ -114,7 +108,7 @@ module ExternalInvariants {
 
     method Update(x: int) 
       requires AllValid()
-      requires Valid() // Should follow automatically since this extends Validatable but ¯\_(ツ)_/¯
+      requires Valid()
       modifies Repr
       ensures AllValid()
     {
@@ -124,10 +118,12 @@ module ExternalInvariants {
       // SomeOtherExternalMethod();
       
       // And this fails because `this` is not `Valid()` at this point
-      // AllStillValid();
+      AllValidatablesUnchanged();
+      AllStillValid();
       
       this.y := 2*x;
 
+      AllValidatablesUnchanged();
       AllStillValid();
       SomeOtherExternalMethod();
     }
@@ -141,9 +137,10 @@ module ExternalInvariants {
   }
 
   method MakeExternalNotAtomic() returns (res: AsExternalNotAtomic)
-    ensures forall o: Validatable :: allocated(o) && fresh(o) && o.P() ==> o.Valid()
+    requires AllValid()
     ensures res.Valid()
     ensures fresh(res.Repr)
+    ensures AllValid()
   {
     var internal := new NotAtomic(73);
     res := new AsExternalNotAtomic(internal);
@@ -154,12 +151,13 @@ module ExternalInvariants {
     predicate Valid() 
       reads this, Repr 
       ensures Valid() ==> this in Repr
-      ensures Valid() ==> forall v :: v in Repr ==> v.Repr <= Repr
+      ensures Valid() ==> forall v :: v in Repr ==> v in AllValidatables() && v.Repr <= Repr
       ensures Valid() ==> forall v :: v in Repr && v != this ==> this !in v.Repr
     {
       && wrapped in Repr
       && Repr == {this} + wrapped.Repr
       && wrapped.Valid()
+      && Repr <= AllValidatables()
     }
 
     twostate lemma IndependentValidity()
@@ -167,18 +165,18 @@ module ExternalInvariants {
       requires unchanged(this)
       requires forall v :: v in Repr && v != this ==> v.Valid()
       ensures Valid()
-    {
-
-    }
+    {}
 
     constructor(wrapped: NotAtomic) 
       requires wrapped.Valid() 
-      ensures forall o: Validatable :: allocated(o) && fresh(o) && o.P() ==> o.Valid()
+      requires wrapped in AllValidatables()
       ensures Valid() 
       ensures fresh(Repr - wrapped.Repr)
     {
       this.wrapped := wrapped;
       this.Repr := {this} + wrapped.Repr;
+      new;
+      RegisterExternallyValid(this);
     }
     method Update(x: int) 
       requires AllValid()
