Test/dafny0/List.dfy
@@ -1,37 +1,98 @@
-class ArrayList<T(0)> {
+trait List {
+  predicate Valid()
+    reads this, Repr
+    ensures Valid() ==> this in Repr
+  ghost var Repr: set<object>
 
-  var data: array<T>
-  var count: int
+  ghost var values: seq<int>
+
+  function method Length(): int
+    requires Valid()
+    reads this, Repr
+    ensures Length() == |values|
+  
+  method Get(i: int) returns (res: int)
+    requires Valid()
+    requires 0 <= i < Length()
+    ensures res == values[i]
+  
+  method Set(i: int, element: int)
+    requires Valid()
+    requires 0 <= i < Length()
+    modifies Repr
+    ensures values == old(values[..i]) + [element] + old(values[i + 1..])
+  
+  method Add(element: int)
+    requires Valid()
+    modifies Repr
+    ensures values == old(values) + [element]
+}
+
+class ArrayList extends List {
+
+  var data: array<int>
+  var length: int
 
   constructor() {
-    data := new T[10];
-    count := 0;
+    data := new int[10];
+    length := 0;
   }
 
-  predicate Valid() reads this {
-    && 0 < data.Length
-    && 0 <= count <= data.Length
-  }
-
-  method Add(t: T) 
-    requires Valid()
-    modifies this, data
+  predicate Valid()
+    reads this, Repr
+    ensures Valid() ==> this in Repr
   {
-    if count == data.Length {
+    && Repr == {this, data}
+    && 0 < data.Length
+    && 0 <= length <= data.Length
+    && values == data[..length]
+  }
+
+  function method Length(): int
+    requires Valid()
+    reads this, Repr
+    ensures Length() == |values|
+  {
+    length
+  }
+  
+  method Get(i: int) returns (res: int)
+    requires Valid()
+    requires 0 <= i < Length()
+    ensures res == values[i]
+  {
+    res := data[i];
+  }
+
+  method Set(i: int, element: int)
+    requires Valid()
+    requires 0 <= i < Length()
+    modifies Repr
+    ensures values == old(values[..i]) + [element] + old(values[i + 1..])
+  {
+    data[i] := element;
+  }
+
+  method Add(element: int)
+    requires Valid()
+    modifies Repr
+    ensures values == old(values) + [element]
+  {
+    if length == data.Length {
       Grow();
     }
-    data[count] := t;
-    count := count + 1;
+    data[length] := element;
+    length := length + 1;
   }
 
   method Grow() 
     requires Valid()
     modifies this`data, data
-    ensures count < data.Length
+    ensures length < data.Length
     ensures fresh(data)
   {
     var oldSize := data.Length;
-    var newData := new T[2 * data.Length];
+    var newData := new int[2 * data.Length];
     forall i | 0 <= i < oldSize {
       newData[i] := data[i];
     }
